fr.inria.atlanmod.coqtl.coq/core/Engine.v
@@ -32,21 +32,15 @@ Require Import Bool.
 Require Import core.utils.Utils.
 Require Import core.Model.
 Require Import core.EqDec.
+Require Import core.TransformationConfiguration.
 
 Scheme Equality for list.
 
 Set Implicit Arguments.
-
-
-
-Class TransformationEngine (SourceModelElement SourceModelLink TargetModelElement TargetModelLink: Type) :=
+  
+Class TransformationEngine (tc: TransformationConfiguration) :=
   {
-
-    eqdec_sme: EqDec SourceModelElement;
-
-    SourceModel := Model SourceModelElement SourceModelLink;
-    TargetModel := Model TargetModelElement TargetModelLink;
-
+    (** ** Syntax *)
     Transformation: Type;
     Rule: Type;
     OutputPatternElement: Type;
@@ -236,7 +230,7 @@ Class TransformationEngine (SourceModelElement SourceModelLink TargetModelElemen
       resolve tls sm name sp iter = return x ->
        (exists (tl : TraceLink),
          In tl tls /\
-         Is_true (list_beq SourceModelElement core.EqDec.eq_b (TraceLink_getSourcePattern tl) sp) /\
+         Is_true (list_beq SourceModelElement SourceElement_eqb (TraceLink_getSourcePattern tl) sp) /\
          ((TraceLink_getIterator tl) = iter) /\ 
          ((TraceLink_getName tl) = name)%string /\
          (TraceLink_getTargetElement tl) = x);
