fr.inria.atlanmod.coqtl.coq/core/Semantics.v
@@ -6,18 +6,13 @@ Require Import core.Syntax.
 Require Import core.EqDec. 
 Require Import Bool.
 Require Import Arith.
+Require Import TransformationConfiguration.
 Scheme Equality for list.
 
 
 Section Semantics.
 
-  Context {SourceModelElement SourceModelLink: Type}.
-  Context {eqdec_sme: EqDec SourceModelElement}. (* need decidable equality on source model elements *)
-  Context {TargetModelElement TargetModelLink: Type}.
-
-  Definition SourceModel := Model SourceModelElement SourceModelLink.
-  Definition TargetModel := Model TargetModelElement TargetModelLink.
-  Definition Transformation := @Transformation SourceModelElement SourceModelLink TargetModelElement TargetModelLink.
+  Context {tc: TransformationConfiguration}.
 
   (*Definition Expr1 (A: Type) (B: Type) : Type := A -> B.
   Definition Expr2 (A: Type) (B: Type) (C: Type) : Type := A -> B -> C.
@@ -42,24 +37,24 @@ Section Semantics.
   Definition evalExpr {A B:Type} (f: Expr A B) (a: A) := f a.
 
   Definition evalGuardExpr' (r : Rule) (sm: SourceModel) (sp: list SourceModelElement) : option bool :=
-  evalExpr (@Rule_getGuardExpr SourceModelElement SourceModelLink TargetModelElement TargetModelLink r) sm sp.
+  evalExpr (Rule_getGuardExpr r) sm sp.
 
   Definition evalIteratorExpr (r : Rule) (sm: SourceModel) (sp: list SourceModelElement) :
     nat :=
-    match (evalExpr (@Rule_getIteratorExpr SourceModelElement SourceModelLink TargetModelElement TargetModelLink r) sm sp) with
+    match (evalExpr (Rule_getIteratorExpr r) sm sp) with
     | Some n => n
     | _ => 0
     end.
 
   Definition evalOutputPatternElementExpr (sm: SourceModel) (sp: list SourceModelElement) (iter: nat) (o: OutputPatternElement)
     : option TargetModelElement := 
-  (evalExpr (@OutputPatternElement_getElementExpr SourceModelElement SourceModelLink TargetModelElement TargetModelLink o) iter sm sp).
+  (evalExpr (OutputPatternElement_getElementExpr o) iter sm sp).
 
   Definition evalOutputPatternLinkExpr
              (sm: SourceModel) (sp: list SourceModelElement) (oe: TargetModelElement) (iter: nat) (tr: list TraceLink)
              (o: OutputPatternElementReference)
     : option TargetModelLink :=
-  (evalExpr (@OutputPatternElementReference_getLinkExpr SourceModelElement SourceModelLink TargetModelElement TargetModelLink o) tr iter sm sp oe).
+  (evalExpr (OutputPatternElementReference_getLinkExpr o) tr iter sm sp oe).
 
   (** * Instantiate **)
 
@@ -118,13 +113,11 @@ Section Semantics.
   Definition trace (tr: Transformation) (sm : SourceModel) : list TraceLink :=
     flat_map (tracePattern tr sm) (allTuples tr sm).  
 
-  Definition TraceLink' := @TraceLink SourceModelElement TargetModelElement.
-
-  Definition resolveIter' (tls: list TraceLink') (sm: SourceModel) (name: string)
+  Definition resolveIter' (tls: list TraceLink) (sm: SourceModel) (name: string)
              (sp: list SourceModelElement)
              (iter : nat) : option TargetModelElement :=
   let tl := find (fun tl: TraceLink => 
-    (list_beq SourceModelElement core.EqDec.eq_b (TraceLink_getSourcePattern tl) sp) &&
+    (list_beq SourceModelElement SourceElement_eqb (TraceLink_getSourcePattern tl) sp) &&
     ((TraceLink_getIterator tl) =? iter) &&
     ((TraceLink_getName tl) =? name)%string) tls in
   match tl with
@@ -158,7 +151,6 @@ Section Semantics.
     | Some sp' => resolveAll' tr sm name sp'
     | None => None
     end.
-
 
   (** * Apply **)
 
